update proofs

Determinism.v
@@ -16,9 +16,108 @@ Require Import Effects.
 Require Import Environment.
 Require Import TypeSystem.
 Require Import Definitions2.
+Require Import CorrectnessLemmas.
 
 Import TypeSoundness.
 
+Inductive Atom_Heap : (DynamicAction * Heap) -> Prop :=
+| PH_Alloc : forall r l v (heap : Heap), Atom_Heap (DA_Alloc r l, update_H ((r,l), v) heap)
+| PH_Read : forall r l v (heap : Heap), find_H (r,l) heap = Some v -> Atom_Heap (DA_Read r l, heap)                                                
+| PH_Write : forall r l v (heap : Heap), find_H (r,l) heap = Some v -> Atom_Heap (DA_Write r l, update_H ((r, l), v) heap). 
+
+Inductive Phi_Heap : (Phi * Heap) -> (Phi * Heap) -> Prop :=
+| PH_Nil    : forall heap,
+                Phi_Heap (Phi_Nil, heap) (Phi_Nil, heap)
+| PH_Atom   : forall i heap',
+                Atom_Heap (i, heap') ->
+                forall phi heap, Phi_Heap (Phi_Seq (Phi_Elem i) phi, heap)  (phi, heap') 
+| PH_Seq_1  : forall phi1 phi1' heap heap',
+                Phi_Heap (phi1, heap) (phi1', heap') ->
+                forall phi2, Phi_Heap (Phi_Seq phi1 phi2, heap)  (Phi_Seq phi1' phi2, heap')
+| PH_Seq_2  : forall phi2 phi2' heap heap',
+                Phi_Heap (phi2, heap) (phi2', heap') ->
+                forall phi1, Phi_Heap (Phi_Seq phi1 phi2, heap)  (Phi_Seq phi1 phi2', heap')
+| PH_Seq_3  : forall phi2 phi2' heap heap',
+                Phi_Heap (phi2, heap) (phi2', heap') ->
+                Phi_Heap (Phi_Seq Phi_Nil phi2, heap)  (Phi_Seq Phi_Nil phi2', heap')
+| PH_Seq_4  : forall heap,
+                Phi_Heap (Phi_Seq Phi_Nil Phi_Nil, heap)  (Phi_Par Phi_Nil Phi_Nil, heap)
+| PH_Par_1  : forall phi1 phi1' heap heap',
+                Phi_Heap (phi1, heap) (phi1', heap') ->
+                forall phi2, Phi_Heap (Phi_Par phi1 phi2, heap)  (Phi_Par phi1' phi2, heap')
+| PH_Par_2  : forall phi2 phi2' heap heap',
+                Phi_Heap (phi2, heap) (phi2', heap') ->
+                forall phi1, Phi_Heap (Phi_Par phi1 phi2, heap)  (Phi_Par phi1 phi2', heap')
+| PH_Par_3  : forall phi2 phi2' heap heap',
+                Phi_Heap (phi2, heap) (phi2', heap') ->
+                Phi_Heap (Phi_Par Phi_Nil phi2, heap)  (Phi_Par Phi_Nil  phi2', heap')
+| PH_Par_4  : forall heap,
+                Phi_Heap (Phi_Par Phi_Nil Phi_Nil, heap)  (Phi_Par Phi_Nil Phi_Nil, heap).                         
+                        
+
+Lemma unique_heap :
+  forall (eff1 eff2 e1 e2: Expr) (heap heap_mu1 heap_mu2 heap_a heap_b : Heap)
+         (env : Env) (rho : Rho) (acts_eff1 acts_eff2 acts_mu1 acts_mu2: Phi)
+         (v1 v2 : Val) (theta1 theta2 : Theta),
+                        (heap, env, rho, eff1) ⇓ (heap, Eff theta1, acts_eff1) ->
+                        (heap, env, rho, eff2) ⇓ (heap, Eff theta2, acts_eff2) ->
+                        (heap, env, rho, e1) ⇓ (heap_mu1, v1, acts_mu1) ->
+                        (heap, env, rho, e2) ⇓ (heap_mu2, v2, acts_mu2) ->
+                        acts_mu1 ⊑ theta1 ->
+                        acts_mu2 ⊑ theta2 ->
+                        Disjointness theta1 theta1 /\ not (Conflictness theta1 theta2) ->
+                        Phi_Heap (Phi_Par acts_mu1 acts_mu2, heap)  (Phi_Par Phi_Nil Phi_Nil, heap_a) -> 
+                        Phi_Heap (Phi_Seq acts_mu1 acts_mu2, heap)  (Phi_Seq Phi_Nil Phi_Nil, heap_b) ->
+                        heap_a = heap_b.
+Proof.
+  intros eff1 eff2 e1 e2
+         heap heap_mu1 heap_mu2 heap_a heap_b
+         env rho
+         acts_eff1 acts_eff2 acts_mu1 acts_mu2
+         v1 v2
+         theta1 theta2.
+  intros H1 H2 H3 H4 H5 H6 H7 H8 H9.
+  generalize dependent eff1.
+  generalize dependent eff2.
+  generalize dependent theta1.
+  generalize dependent theta2.
+  generalize dependent heap_a.
+  generalize dependent heap_b. 
+  generalize dependent acts_eff2.
+  generalize dependent acts_eff1.
+  induction acts_mu1, acts_mu2;
+    try (solve [ intros acts_eff1 acts_eff2 heap_b HPhi2 heap_a HPhi1;
+                 intros theta2 HTheta2 theta1 HTheta1;
+                 intros HDisj; intros eff2 HEff2 eff1 HEff1;
+                 inversion HPhi1; subst; inversion HPhi2; subst
+               | intros acts_eff1 acts_eff2 heap_b HPhi2 heap_a HPhi1;
+                 intros theta2 HTheta2 theta1 HTheta1;
+                 intros HDisj; intros eff2 HEff2 eff1 HEff1;
+                 inversion HPhi1; subst; inversion HPhi2; subst;
+                 inversion H1; inversion H0; subst
+               | intros acts_eff1 acts_eff2 heap_b HPhi2 heap_a HPhi1;
+                 intros theta2 HTheta2 theta1 HTheta1;
+                 intros HDisj; intros eff2 HEff2 eff1 HEff1;
+                 inversion HPhi1; subst; inversion HPhi2; subst;
+                 try (solve [inversion H1; inversion H0; subst; symmetry; assumption | inversion H0; subst; reflexivity])
+               ]).
+  - intros acts_eff1 acts_eff2 heap_b HPhi2 heap_a HPhi1;
+    intros theta2 HTheta2 theta1 HTheta1;
+    intros HDisj; intros eff2 HEff2 eff1 HEff1;
+    inversion HPhi1; subst; inversion HPhi2; subst;
+    inversion H1; inversion H0; subst; inversion H9; subst.
+    + admit.
+    + admit.
+    + admit.
+    + admit.
+  - intros acts_eff1 acts_eff2 heap_b HPhi2 heap_a HPhi1;
+    intros theta2 HTheta2 theta1 HTheta1;
+    intros HDisj; intros eff2 HEff2 eff1 HEff1;
+    inversion HPhi1; subst; inversion HPhi2; subst.
+    inversion H1; inversion H0; subst; inversion H9; subst.
+    admit.
+Qed.        
+    
 
 
 Theorem DynamicDeterminism :
